Hnr_Diff_Arr.thy
@@ -4,65 +4,94 @@ begin
 
 named_theorems hnr_rule_diff_arr
 
+definition master_assn' where
+  "master_assn' S = (\<exists>\<^sub>At. master_assn t * \<up>(\<forall> (xs, xsi) \<in> S. t \<turnstile> xs \<sim> xsi))"
+
 lemma hnr_copy_diff_arr [hnr_rule_diff_arr]:
-  "hnr (master_assn t * \<up>(t \<turnstile> x \<sim> xi)) (return xi) (\<lambda>x xi. master_assn t * \<up>(t \<turnstile> x \<sim> xi)) x"
+  "hnr 
+      (master_assn' (insert (xs, xsi) S)) 
+      (return xsi) 
+      (\<lambda>xs' xsi'. master_assn' (insert (xs', xsi') S)) 
+      xs"
   apply(rule hnrI)
+  unfolding master_assn'_def
   by sep_auto
 
-lemma hnr_from_array: 
+definition Diff_Arr_From_Arr where
+  "Diff_Arr_From_Arr a = a"
+
+lemma hnr_from_array [hnr_rule_diff_arr]: 
   "hnr 
     (array_assn xs xsi)
     (Diff_Arr.from_array xsi)
-    (\<lambda>xs xsi. \<exists>\<^sub>At. master_assn t * \<up>(t \<turnstile> xs \<sim> xsi))
-    xs
+    (\<lambda>xs xsi. master_assn' { (xs, xsi) })
+    (Diff_Arr_From_Arr xs)
   "
   apply(rule hnrI)
-  using ent_refl_true fi_rule from_array by blast
+  unfolding master_assn'_def Diff_Arr_From_Arr_def
+  by sep_auto
 
-lemma hnr_from_list: 
+definition New_Diff_Arr where
+  "New_Diff_Arr a = a"
+
+lemma hnr_from_list [hnr_rule_diff_arr]: 
   "hnr 
     emp
     (Diff_Arr.from_list xs)
-    (\<lambda>xs xsi. \<exists>\<^sub>At. master_assn t * \<up>(t \<turnstile> xs \<sim> xsi))
-    xs
+    (\<lambda>xs xsi. master_assn' { (xs, xsi) })
+    (New_Diff_Arr xs)
   "
   apply(rule hnrI)
-  using ent_refl_true fi_rule from_list by blast
+  unfolding master_assn'_def New_Diff_Arr_def
+  by sep_auto
 
 lemma hnr_lookup[hnr_rule_diff_arr]: "
   hnr
-    (master_assn t * id_assn i ii * \<up>(t \<turnstile> xs \<sim> xsi))
+    (master_assn' (insert (xs, xsi) S) * id_assn i ii) 
     (diff_arr_lookup_safe xsi ii)
-    (\<lambda>r ri. master_assn t * id_assn r ri)
+    (\<lambda>r ri. id_assn r ri * master_assn' S)
     (xs ! i)"
-  unfolding id_rel_def
+  unfolding id_rel_def master_assn'_def
   apply(rule hnrI)
-  using lookup_safe by fastforce
+  apply sep_auto
+  subgoal for t
+    apply(subgoal_tac "t \<turnstile> xs  \<sim> xsi")
+     apply(rule cons_post_rule)
+   apply(rule fi_rule[OF lookup_safe[of t xs]])
+    by sep_auto+
+  done
 
 lemma hnr_realize: "
   hnr
-    (master_assn t * \<up>(t \<turnstile> xs \<sim> xsi))
+    (master_assn' (insert (xs, xsi) S))
     (Diff_Arr.realize xsi)
-    (\<lambda> r ri. master_assn t  * array_assn r ri)
+    (\<lambda> r ri. master_assn' S * array_assn r ri)
     xs"
-  unfolding id_rel_def
+  unfolding id_rel_def master_assn'_def
   apply(rule hnrI)
-  using realize[of t xs xsi]
-  by(sep_auto simp: cons_post_rule ent_refl_true)
+  apply sep_auto
+  subgoal for t
+    apply(subgoal_tac "t \<turnstile> xs  \<sim> xsi")
+     apply(rule cons_post_rule)
+   apply(rule fi_rule[OF realize[of t xs]])
+    by sep_auto+
+  done
 
 lemma hnr_update[hnr_rule_diff_arr]: "
   hnr
-    (master_assn t * \<up>(t \<turnstile> xs \<sim> xsi) * id_assn i ii * id_assn v vi)
+    (master_assn' (insert (xs, xsi) S) * id_assn i ii * id_assn v vi)
     (diff_arr_update_safe xsi ii vi)
-    (\<lambda>xs xsi. \<exists>\<^sub>At'. master_assn t' * 
-              \<up>((\<forall>xs' xsi'. t \<turnstile> xs' \<sim>  xsi' \<longrightarrow> t' \<turnstile> xs' \<sim>  xsi') \<and> t' \<turnstile> xs \<sim> xsi))
+    (\<lambda>xs' xsi'. master_assn' (insert (xs', xsi') S))
     (xs [i:= v])"
-  unfolding id_rel_def
+  unfolding id_rel_def master_assn'_def
   apply(rule hnrI)
   apply(sep_auto)
-  apply(rule cons_post_rule)
-  apply(rule fi_rule[OF update_safe])
-  by sep_auto+  
+  subgoal for t
+    apply(subgoal_tac "t \<turnstile> xs  \<sim> xsi")
+     apply(rule cons_post_rule)
+   apply(rule fi_rule[OF update_safe[of t xs]])
+    by sep_auto+
+  done
 
 lemma transfer_diff_arr_rel:
   assumes 
@@ -75,17 +104,137 @@ lemma transfer_diff_arr_rel:
 method hnr_transfer_diff_arr_rel = 
   ((drule(1) transfer_diff_arr_rel)+)?, (thin_tac "\<forall>xs' xsi'. _ \<turnstile> xs' \<sim> xsi' \<longrightarrow> _ \<turnstile> xs' \<sim> xsi'")
 
-method hnr_diff_arr = hnr hnr_transfer_diff_arr_rel rule_set: hnr_rule_diff_arr
+definition Si_Tag where
+  "Si_Tag x = x"
 
-lemma bug_1: 
-  assumes "master_assn t \<Longrightarrow>\<^sub>A \<exists>\<^sub>Ax. master_assn x"
-  shows "master_assn t \<Longrightarrow>\<^sub>A \<exists>\<^sub>Ax. master_assn x"
+lemma si_initialize: "A \<union> {} = Si_Tag B \<Longrightarrow> A = B"
+  unfolding Si_Tag_def
+  by simp
+
+lemma si_move_tag: "Si_Tag (insert x B) = insert x (Si_Tag B)"
+  unfolding Si_Tag_def
+  by simp
+
+lemma si_rotate: "A \<union> insert x B = C \<Longrightarrow> insert x A \<union> B = C"
+  by simp
+
+lemma si_match: "insert x A \<union> B = C \<Longrightarrow> insert x A \<union> B = insert x C"
+  by auto
+
+lemma si_rotate_back: "insert x A \<union> B = C \<Longrightarrow> A \<union> insert x B = C"
+  by simp
+
+lemma si_finish: "A \<union> {} = Si_Tag A"
+  unfolding Si_Tag_def
+  by simp
+
+method si_try_match = then_else 
+  \<open>rule si_match\<close>
+  \<open>((rule si_rotate_back)+)?\<close>
+  \<open>rule si_rotate, si_try_match\<close>
+
+method si_initialize = rule si_initialize, (simp(no_asm) only: si_move_tag)?
+
+method set_inference_keep = si_initialize, ((rule si_finish | si_try_match)+)?
+
+method set_inference = set_inference_keep; fail
+
+experiment
+begin
+
+schematic_goal "{ 1, 2, 3 } = ?S"
+  apply set_inference
+  done
+
+schematic_goal "{ 1, 2, 3 } = insert 3 (insert 2 ?S)"
+  apply set_inference
+  done
+
+schematic_goal "{ 1, 2, 3 } = insert 1 (insert 2 (insert 3 ?S))"
+  apply set_inference
+  done
+
+schematic_goal "{ 1, 2, 3 } = insert 4 (insert 2 (insert 4 ?S))"
+  apply set_inference_keep
+  oops
+
+end
+
+lemma master_assn'_cong:
+  assumes
+    "S = S'"
+  shows 
+    "master_assn' S \<Longrightarrow>\<^sub>A master_assn' S'"
   using assms
-  sorry
+  by simp
 
-lemma bug_2: "master_assn t \<Longrightarrow>\<^sub>A \<exists>\<^sub>Ax. master_assn x"
-  using triv_exI[of master_assn t]
-  apply auto
-  sorry
+method hnr_diff_arr_match_atom = then_else
+  \<open>rule master_assn'_cong\<close>
+  \<open>set_inference\<close>
+  \<open>rule ent_refl\<close>
+
+lemma kdm_init: 
+  assumes
+    "S' \<subseteq> S"
+    "S' = S'"
+  shows
+    "master_assn' S \<Longrightarrow>\<^sub>A master_assn' S'"
+  using assms
+  unfolding master_assn'_def
+  by sep_auto
+
+lemma kdm_keep:
+  assumes
+    "S' \<subseteq> S"
+  shows
+    "insert x S' \<subseteq> insert x S"
+  using assms
+  by auto
+
+lemma kdm_drop:
+  assumes
+    "S' \<subseteq> S"
+  shows
+    "S' \<subseteq> insert x S"
+  using assms
+  by auto
+
+
+method kdm_subset = ((rule kdm_keep | rule kdm_drop)+)?, rule subset_refl
+
+method kdm_check_not_empty = then_else
+  \<open>rule refl[of "{}"]\<close>
+  \<open>fail\<close>
+  \<open>rule refl\<close>
+
+method kdm = rule kdm_init, kdm_subset, kdm_check_not_empty
+
+method diff_arr_kdm = rule ent_refl | kdm
+
+experiment
+begin
+
+schematic_goal "master_assn' ({ a, b, c }:: ('a :: heap list \<times> 'a cell ref) set)
+   \<Longrightarrow>\<^sub>A master_assn' (?S :: ('a list \<times> 'a cell ref) set)"
+  apply kdm
+  done
+
+schematic_goal 
+  "\<And> a b c. master_assn' ({ a, b, c }:: ('a :: heap list \<times> 'a cell ref) set)
+   \<Longrightarrow>\<^sub>A master_assn' (?S :: ('a list \<times> 'a cell ref) set)"
+  apply(then_else kdm fail succeed)
+  oops
+
+schematic_goal 
+  "\<And> a b c. master_assn' ({ a, b, c }:: ('a :: heap list \<times> 'a cell ref) set)
+   \<Longrightarrow>\<^sub>A master_assn' (?S a c :: ('a list \<times> 'a cell ref) set)"
+  apply kdm
+  done
+
+end
+  
+method hnr_diff_arr = hnr hnr_diff_arr_match_atom diff_arr_kdm rule_set: hnr_rule_diff_arr
+
+method hnr_step_diff_arr = hnr_step hnr_diff_arr_match_atom diff_arr_kdm rule_set: hnr_rule_diff_arr
 
 end
