Test_Hnr.thy
@@ -2,179 +2,314 @@ theory Test_Hnr
   imports Hnr_Diff_Arr Hnr_Array "HOL-Library.Code_Target_Nat" 
 begin
 
-definition test1 where
-  "test1 xs = 
-    (let c1 = (let x = 1 in x); c2 = 2; c3 = 3; t1 = xs[c1 := c2]; t2 = t1[c1 := c3]; t3 = t2 ! c2 in t3)"
+definition sequential_1 where
+  "sequential_1 xs = 
+    (let c1 = (let x = 1 in x); 
+         c2 = 2; 
+         c3 = 3; 
+         t1 = xs[c1 := c2]; 
+         t2 = t1[c1 := c3];
+         t3 = t2 ! c2 
+      in t3)"
 
-definition test2 where
-  "test2 xs = 
+definition sequential_2 where
+  "sequential_2 xs = 
     (let c1 = 1; t1 = xs[c1 := c1] in t1)"
 
-definition test2_1 where
-  "test2_1 xs = 
-    (let c1 = 1; t1 = xs[c1 := c1] in (c1, t1))"
-
-definition test2_2 where
-  "test2_2 xs = 
-    (let c1 = 1; t1 = xs; t2 = xs[c1 := c1] in (t1, t2))"
-
-definition test2_3 where
-  "test2_3 xs = 
+definition return_tuple_1 where
+  "return_tuple_1 xs = 
     (let c1 = 1; c2 = 2 in (c1, c2))"
 
-definition test3 where
-  "test3 xs = 
+definition return_tuple_2 where
+  "return_tuple_2 xs = 
+    (let c1 = 1; t1 = xs[c1 := c1] in (c1, t1))"
+
+definition return_tuple_3 where
+  "return_tuple_3 xs = 
+    (let c1 = 1; t1 = xs; t2 = xs[c1 := c1] in (t1, t2))"
+
+definition not_linear where
+  "not_linear xs = 
     (let c1 = 1; t1 = xs[c1 := c1]; t2 = xs ! c1 in t1)"
 
-definition test4 where
-  "test4 xs =
-    (let c1 = 1; t1 = if xs = [] then xs else let t2 = xs[c1 := c1] in t2 in t1)"
+definition if_1 where
+  "if_1 xs =
+    (let c1 = 1; 
+         t1 = if xs = [] 
+              then xs 
+              else let t2 = xs[c1 := c1]
+                   in t2 
+     in t1)"
 
-definition test4_2 where
-  "test4_2 xs =
-    (let c1 = 1; t1 = if xs = [] then xs else let t1 = xs[c1 := c1]; t2 = t1[c1:= c1] in t2 in t1)"
+definition if_2 where
+  "if_2 xs =
+    (let c1 = 1; 
+         t1 = if xs = [] 
+              then xs 
+              else let t1 = xs[c1 := c1]; 
+                       t2 = t1[c1:= c1] 
+                   in t2 
+      in t1)"
 
-definition test4_3 where
-  "test4_3 xs =
-    (let c1 = 1; t1 = if xs = [] then let c2 = 2; t1 = xs[c2 := c2]; t2 = t1[c2:= c2] in xs else let t1 = xs[c1 := c1]; t2 = t1[c1:= c1] in t2 in t1)"
+definition if_3 where
+  "if_3 xs =
+    (let c1 = 1; 
+         t1 = if xs = [] 
+              then let c2 = 2; t1 = xs[c2 := c2]; t2 = t1[c2:= c2] 
+                   in xs 
+              else let t1 = xs[c1 := c1]; t2 = t1[c1:= c1] 
+                   in t2 
+     in t1)"
 
-(* TODO: What to do if the bool depends on local variables? *)
-definition test5 where
-  "test5 xs = 
-    (let c1 = 1; t1 = if c1 = 0 then xs else xs[c1 := c1] in t1)"
+definition if_4 where
+  "if_4 xs = 
+    (let c1 = 1; t1 = if True then xs else xs[c1 := c1] in t1)"
 
-(* TODO: I need this form but need to find a way for comparisons *)
-definition test5_1 where
-  "test5_1 xs = 
+definition if_5 where
+  "if_5 xs = 
+    (let c1 = 1; 
+         c2 = 2; 
+         t1 = if xs = [] 
+              then xs[c2 := c2] 
+              else xs[c1 := c1] 
+     in t1)"
+
+definition if_6 where
+  "if_6 xs = 
+    (let c1 = 1; 
+         c2 = 2; 
+         t1 = if xs = [] 
+              then let t2 = xs[c2 := c2]; t3 = xs[c1 := c1] in t3 
+              else let t2 = xs[c1 := c1]; t3 = xs[c2 := c1] in t3 
+         in t1)"
+
+definition if_7 where
+  "if_7 xs ys = (
+    let c1 = 1 
+    in if xs = [] 
+       then let t1 = xs[c1 := c1]; t2 = ys[c1 := c1] 
+            in (t1, t1) 
+       else let t1 = ys[c1 := c1] 
+            in (t1, t1)
+    )"
+
+definition fallback_1 where
+  "fallback_1 xs = 
     (let c1 = 1; b = (c1 = c1); t1 = if b then xs else xs[c1 := c1] in t1)"
 
-definition test6 where
-  "test6 xs = 
-    (let c1 = 1; c2 = 2; t1 = if xs = [] then xs[c2 := c2] else xs[c1 := c1] in t1)"
+definition create_list where
+  "create_list x = [x]" 
 
-definition test7 where
-  "test7 xs = 
-    (let c1 = 1; c2 = 2; t1 = if xs = [] then let t2 = xs[c2 := c2]; t3 = xs[c1 := c1] in t3 else let t2 = xs[c1 := c1]; t3 = xs[c2 := c1] in t3 in t1)"
+definition create_arr where
+  "create_arr xs = New_Arr [xs]"
 
+definition create_diff_arr_empty where
+  "create_diff_arr_empty = New_Diff_Arr []" 
 
-schematic_goal "hnr (array_assn xs xsi) (?c :: ?'a Heap) ?\<Gamma>' (test1 xs)"
-  unfolding test1_def 
-  apply hnr_arr
-  done
+definition create_diff_arr where
+  "create_diff_arr x = New_Diff_Arr [x]" 
 
-schematic_goal "hnr (array_assn xs xsi) (?c :: ?'a Heap) ?\<Gamma>' (test2 xs)"
-  unfolding test2_def 
-  apply hnr_arr
-  done  
+definition create_diff_arr_2 where
+  "create_diff_arr_2 xs = (let a = New_Diff_Arr [xs]; b = New_Diff_Arr [a] in b)" 
 
-schematic_goal "hnr (array_assn xs xsi) (?c :: ?'a Heap) ?\<Gamma>' (test2_1 xs)"
-  unfolding test2_1_def 
-  apply hnr_arr
-  done  
+definition create_diff_arr_3 where
+  "create_diff_arr_3 = (let xs = New_Diff_Arr [] in xs)"
 
-schematic_goal "hnr (array_assn xs xsi) (?c :: ?'a Heap) ?\<Gamma>' (test2_3 xs)"
-  unfolding test2_3_def 
-  apply hnr_arr
-  done  
+definition create_arr_diff_arr where
+  "create_arr_diff_arr xs = (let a = New_Arr [xs]; b = Diff_Arr_From_Arr a in b)" 
+
+definition case_tuple where
+  "case_tuple x = (case x of (x1, x2) \<Rightarrow> let c = x2 in x1)"
+
+definition case_nat where
+  "case_nat n = (case n of 
+                        0 \<Rightarrow> let xs = New_Diff_Arr [] in xs 
+                  | Suc n \<Rightarrow> let xs = New_Diff_Arr [] in xs)"
+
+(* HNR Array *)
+
+schematic_goal "hnr (array_assn xs xsi) (?c :: ?'a Heap) ?\<Gamma>' (sequential_1 xs)"
+  unfolding sequential_1_def 
+  by hnr_arr
+
+schematic_goal "hnr (array_assn xs xsi) (?c :: ?'a Heap) ?\<Gamma>' (sequential_2 xs)"
+  unfolding sequential_2_def 
+  by hnr_arr
+
+schematic_goal "hnr (array_assn xs xsi) (?c :: ?'a Heap) ?\<Gamma>' (return_tuple_1 xs)"
+  unfolding return_tuple_1_def
+  by hnr_arr
+
+(* TODO: Why is id_assn duplicated ? *)
+schematic_goal "hnr (array_assn xs xsi) (?c :: ?'a Heap) ?\<Gamma>' (return_tuple_2 xs)"
+  unfolding return_tuple_2_def 
+  by hnr_arr
 
 (* Can't work, not linear! *)
-schematic_goal "hnr (array_assn xs xsi) (?c :: ?'a Heap) ?\<Gamma>' (test3 xs)"
-  unfolding test3_def 
+schematic_goal "hnr (array_assn xs xsi) (?c :: ?'a Heap) ?\<Gamma>' (return_tuple_3 xs)"
+  unfolding return_tuple_3_def 
   apply hnr_arr
+  oops  
+
+(* Can't work, not linear! *)
+schematic_goal "hnr (array_assn xs xsi) (?c :: ?'a Heap) ?\<Gamma>' (not_linear xs)"
+  unfolding not_linear_def 
+  apply hnr_arr
+  oops 
+
+schematic_goal "hnr (array_assn xs xsi) (?c :: ?'a Heap) ?\<Gamma>' (if_1 xs)"
+  unfolding if_1_def 
+  by hnr_arr
+
+schematic_goal "hnr (array_assn xs xsi) (?c :: ?'a Heap) ?\<Gamma>' (if_2 xs)"
+  unfolding if_2_def 
+  by hnr_arr
+
+schematic_goal "hnr (array_assn xs xsi) (?c :: ?'a Heap) ?\<Gamma>' (if_3 xs)"
+  unfolding if_3_def 
+  by hnr_arr
+
+schematic_goal "hnr (array_assn xs xsi) (?c :: ?'a Heap) ?\<Gamma>' (if_4 xs)"
+  unfolding if_4_def 
+  by hnr_arr
+
+schematic_goal "hnr (array_assn xs xsi) (?c :: ?'a Heap) ?\<Gamma>' (if_5 xs)"
+  unfolding if_5_def 
+  by hnr_arr
+
+(* TODO: There is something wrong here *)
+schematic_goal "hnr (array_assn xs xsi) (?c :: ?'a Heap) ?\<Gamma>' (if_6 xs)"
+  unfolding if_6_def 
+  by hnr_arr
+
+(* TODO: There is something wrong here *)
+schematic_goal "hnr (array_assn xs xsi) (?c :: ?'a Heap) ?\<Gamma>' (if_7 xs)"
+  unfolding if_7_def 
+  by hnr_arr
+
+(* TODO: Why does this work ? *)
+schematic_goal "hnr (array_assn xs xsi) (?c :: ?'a Heap) ?\<Gamma>' (fallback_1 xs)"
+  unfolding fallback_1_def 
+  by hnr_arr
+
+(* TODO *)
+schematic_goal "hnr emp (?c :: ?'a Heap) ?\<Gamma>' (create_list x)"
+  unfolding create_list_def 
+  by hnr_arr
+
+(* TODO *)
+schematic_goal "hnr emp (?c :: ?'a Heap) ?\<Gamma>' (create_arr x)"
+  unfolding create_arr_def 
+  by hnr_arr
+
+(* TODO *)
+schematic_goal "hnr (id_assn x xi) (?c :: ?'a Heap) ?\<Gamma>' (case_tuple x)"
+  unfolding case_tuple_def
+  by hnr_arr
+
+(* TODO *)
+schematic_goal "hnr (id_assn x xi) (?c :: ?'a Heap) ?\<Gamma>' (case_nat x)"
+  unfolding case_nat_def
+  by hnr_arr
+
+(* HNR Diff-Array *)
+
+schematic_goal "hnr (master_assn' {(xs, xsi)}) (?c :: ?'a Heap) ?\<Gamma>' (sequential_1 xs)"
+  unfolding sequential_1_def 
+  by hnr_diff_arr
+
+schematic_goal "hnr (master_assn' {(xs, xsi)}) (?c :: ?'a Heap) ?\<Gamma>' (sequential_2 xs)"
+  unfolding sequential_2_def 
+  by hnr_diff_arr
+
+schematic_goal "hnr(master_assn' {(xs, xsi)}) (?c :: ?'a Heap) ?\<Gamma>' (return_tuple_1 xs)"
+  unfolding return_tuple_1_def
+  by hnr_diff_arr
+
+(* TODO: Why is there no assn afterwards? *)
+schematic_goal "hnr (master_assn' {(xs, xsi)}) (?c :: ?'a Heap) ?\<Gamma>' (return_tuple_2 xs)"
+  unfolding return_tuple_2_def 
+  by hnr_diff_arr
+
+(* TODO: Why is there no assn afterwards? *)
+schematic_goal "hnr (master_assn' {(xs, xsi)}) (?c :: ?'a Heap) ?\<Gamma>' (return_tuple_3 xs)"
+  unfolding return_tuple_3_def 
+  by hnr_diff_arr
+
+schematic_goal "hnr (master_assn' {(xs, xsi)}) (?c :: ?'a Heap) ?\<Gamma>' (not_linear xs)"
+  unfolding not_linear_def 
+  by hnr_diff_arr
+
+schematic_goal "hnr (master_assn' {(xs, xsi)}) (?c :: ?'a Heap) ?\<Gamma>' (if_1 xs)"
+  unfolding if_1_def 
+  by hnr_diff_arr
+
+schematic_goal "hnr (master_assn' {(xs, xsi)}) (?c :: ?'a Heap) ?\<Gamma>' (if_2 xs)"
+  unfolding if_2_def 
+  by hnr_diff_arr
+
+schematic_goal "hnr (master_assn' {(xs, xsi)}) (?c :: ?'a Heap) ?\<Gamma>' (if_3 xs)"
+  unfolding if_3_def 
+  by hnr_diff_arr
+
+schematic_goal "hnr (master_assn' {(xs, xsi)}) (?c :: ?'a Heap) ?\<Gamma>' (if_4 xs)"
+  unfolding if_4_def 
+  by hnr_diff_arr
+
+schematic_goal "hnr (master_assn' {(xs, xsi)}) (?c :: ?'a Heap) ?\<Gamma>' (if_5 xs)"
+  unfolding if_5_def 
+  by hnr_diff_arr
+
+schematic_goal "hnr (master_assn' {(xs, xsi)}) (?c :: ?'a Heap) ?\<Gamma>' (if_6 xs)"
+  unfolding if_6_def 
+  by hnr_diff_arr
+
+(* TODO: We don't want an id_assn for the tuple, right? *)
+schematic_goal "hnr (master_assn' {(xs, xsi)}) (?c :: ?'a Heap) ?\<Gamma>' (if_7 xs)"
+  unfolding if_7_def 
+  by hnr_diff_arr
+
+(* TODO: Why does this work ? *)
+schematic_goal "hnr (master_assn' {(xs, xsi)}) (?c :: ?'a Heap) ?\<Gamma>' (fallback_1 xs)"
+  unfolding fallback_1_def 
+  by hnr_diff_arr
+
+schematic_goal "hnr emp (?c :: ?'a Heap) ?\<Gamma>' (create_list x)"
+  unfolding create_list_def 
+  by hnr_diff_arr
+
+(* TODO: Doesn't seem to work correctly anymore *)
+schematic_goal "hnr emp (?c :: ?'a Heap) ?\<Gamma>' (create_diff_arr_empty)"
+  unfolding create_diff_arr_empty_def 
+  by hnr_diff_arr
+
+(* TODO: Doesn't seem to work correctly anymore *)
+schematic_goal "hnr emp (?c :: ?'a Heap) ?\<Gamma>' (create_diff_arr x)"
+  unfolding create_diff_arr_def 
+  by hnr_diff_arr
+
+schematic_goal "hnr emp (?c :: ?'a Heap) ?\<Gamma>' (create_diff_arr_2 x)"
+  unfolding create_diff_arr_2_def 
+  by hnr_diff_arr
+                                                 
+schematic_goal "hnr emp (?c :: ?'a Heap) ?\<Gamma>' (create_diff_arr_3)"
+  unfolding create_diff_arr_3_def 
+  by hnr_diff_arr
+
+(* TODO: This worked before the clean up ^^ - Do I need a combined operator? *)
+schematic_goal "hnr emp (?c :: ?'a Heap) ?\<Gamma>' (create_arr_diff_arr x)"
+  unfolding create_arr_diff_arr_def 
+  apply hnr_arr
+  (* apply hnr_diff_arr *)
   sorry
 
-schematic_goal "hnr (master_assn t * \<up>(t \<turnstile> xs \<sim> xsi)) (?c :: ?'a Heap) ?\<Gamma>' (test1 xs)"
-  unfolding test1_def
-  apply hnr_diff_arr
-  done
+schematic_goal "hnr (id_assn x xi) (?c :: ?'a Heap) ?\<Gamma>' (case_tuple x)"
+  unfolding case_tuple_def
+  by hnr_diff_arr
 
-schematic_goal "hnr (master_assn t * \<up>(t \<turnstile> xs \<sim> xsi)) (?c :: ?'a Heap) ?\<Gamma>' (test2 xs)"
-  unfolding test2_def
-  apply hnr_diff_arr
-  done
-
-schematic_goal "hnr (master_assn t * \<up>(t \<turnstile> xs \<sim> xsi)) (?c :: ?'a Heap) ?\<Gamma>' (test2_1 xs)"
-  unfolding test2_1_def
-  apply hnr_diff_arr
-  done
-
-schematic_goal "hnr (master_assn t * \<up>(t \<turnstile> xs \<sim> xsi)) (?c :: ?'a Heap) ?\<Gamma>' (test2_2 xs)"
-  unfolding test2_2_def
-  apply hnr_diff_arr
-  done
-
-schematic_goal "hnr (master_assn t * \<up>(t \<turnstile> xs \<sim> xsi)) (?c :: ?'a Heap) ?\<Gamma>' (test2_3 xs)"
-  unfolding test2_3_def
-  apply hnr_diff_arr
-  done
-
-schematic_goal "hnr (master_assn t * \<up>(t \<turnstile> xs \<sim> xsi)) (?c xsi :: ?'a Heap) (?\<Gamma>' xsi xs) (test3 xs)"
-  unfolding test3_def
-  apply hnr_diff_arr
-  done  
-
-schematic_goal "hnr (master_assn t * \<up>(t \<turnstile> xs \<sim> xsi)) (?c xsi :: ?'a Heap) (?\<Gamma>' xsi xs) (test4 xs)"
-  unfolding test4_def
-  sorry
-  (* apply hnr_diff_arr
-     apply (rule hnr_if)
-      apply hnr_diff_arr
-  subgoal sorry
-  subgoal 
-    apply(rule merge_if_2)
-    apply hnr_diff_arr
-  sorry *)
-
-schematic_goal "hnr (master_assn t * \<up>(t \<turnstile> xs \<sim> xsi)) (?c xsi :: ?'a Heap) (?\<Gamma>' xsi xs) (test4_2 xs)"
-  unfolding test4_2_def
-  apply hnr_diff_arr
-  apply or_match 
-  apply or_match 
-  apply or_match 
-  apply(hnr_extract_pure -)
-  subgoal sorry       
-  subgoal sorry
-  subgoal sorry
-  sorry
-  (* apply hnr_diff_arr
-
-     apply (rule hnr_if)
-      apply hnr_diff_arr
-  apply simp
-    apply(rule merge_if_2)
-    apply hnr_diff_arr
-  done *)
-
-schematic_goal "hnr (master_assn t * \<up>(t \<turnstile> xs \<sim> xsi)) (?c xsi :: ?'a Heap) (?\<Gamma>' xsi xs) (test4_3 xs)"
-  unfolding test4_3_def
-  apply hnr_diff_arr
-  apply or_match+
-  subgoal sorry       
-  subgoal sorry
-  subgoal sorry
-  sorry
-
-schematic_goal "hnr (master_assn t * \<up>(t \<turnstile> xs \<sim> xsi)) (?c xsi :: ?'a Heap) (?\<Gamma>' xsi xs) (test5_1 xs)"
-  unfolding test5_1_def
-  
-  sorry
-
-schematic_goal "hnr (master_assn t * \<up>(t \<turnstile> xs \<sim> xsi)) (?c xsi :: ?'a Heap) (?\<Gamma>' xsi xs) (test7 xs)"
-  unfolding test7_def
-  apply hnr_diff_arr
-  apply or_match+
-  subgoal sorry
-  subgoal sorry
-  subgoal sorry
-  subgoal sorry
-  sorry
-
-(* 
-  Questions/Notes: 
-  - Wouldn't it be more useful to always build up the master_assn instead of using existensials?
-  - How to integrate standard operations like + and -? Bool ops? Simple function call? 
-  - How to integrate Annotations?
-*)
+schematic_goal "hnr (id_assn x xi) (?c :: ?'a Heap) ?\<Gamma>' (case_nat x)"
+  unfolding case_nat_def
+  by hnr_diff_arr
 
 
 export_code array_nth_safe array_update_safe in SML_imp
